{
 "cells": [
  {
   "cell_type": "markdown",
   "metadata": {},
   "source": [
    "# Assignment 3\n",
    "\n",
    "Peder Ørmen Bukaasen, Bård Tollef Pedersen and Eivind Lid Trøen"
   ]
  },
  {
   "cell_type": "markdown",
   "metadata": {},
   "source": [
    "## Exercise 1\n",
    "\n",
    "```\n",
    "def f1(n):\n",
    "    result = [1 for _ in range(10)]  #  constant time c*10\n",
    "    return result\n",
    "``` \n",
    "Here the time complexety is c*10, and can be written as <u>O(1)</u>  \n",
    "\n",
    "```\n",
    "def f2(n):\n",
    "    total = 0\n",
    "    for i in range(n): # c1*n\n",
    "        total += i # constant time c2\n",
    "    return total\n",
    "```\n",
    "Here the time complexety is c1*n+c2, and can be written as <u>O(n)</u>\n",
    "\n",
    "```\n",
    "def f3(n):\n",
    "    matrix = [[0 for _ in range(n)] for _ in range(n)]  # c1*n * c2*n\n",
    "    return matrix\n",
    "```\n",
    "Here the time complexety is c1 * n * c2 * n, and can be written as c3 * n * n wich is equal to <u>O(n^2)</u>\n",
    "\n",
    "\n",
    "```\n",
    "def f4(n):\n",
    "    if n <= 1:  # constant time c1\n",
    "        return n\n",
    "    count = 0\n",
    "    for _ in range(2**n): # c2 * 2^n\n",
    "        for _ in range(2**n): # c3 * 2^n\n",
    "            count += 1 # constant time c4\n",
    "    return count\n",
    "```\n",
    "Here the time complexety is c1 + c2 * 2^n * c3 * 2^n + c4, and can be written as c5 + c6 * 2^n * 2^n, can be written ad c5 + c6 * 4^n wich is equal to <u>O(4^n)</u>\n"
   ]
  },
  {
   "cell_type": "markdown",
   "metadata": {},
   "source": [
    "## Exercise 2"
   ]
  },
  {
   "cell_type": "markdown",
   "metadata": {},
   "source": [
    "Use mathematical induction to show that when  is an exact power of 2, the solution of the recurrence\n",
    "\n",
    "T(n) = {  \n",
    "    1 if n = 1  \n",
    "    8T(n/2) + n<sup>2</sup> if n = 2<sup>k</sup> for k >= 1  \n",
    "}\n",
    "is T(n) = n<sup>2</sup> * (2n - 1)\n",
    "  \n",
    "   \n",
    "First prove that it holds for n=2<sup>1</sup>  \n",
    "\n",
    "T(2<sup>1</sup>) = (2<sup>1</sup>)<sup>2</sup> * (2 * 2<sup>1</sup> -1) = 2<sup>2</sup> * 2<sup>2</sup> - 2<sup>2</sup> = 16 - 4 = 12  \n",
    "T(2<sup>1</sup>) = 8T(2<sup>1</sup> /2) + 2<sup>1</sup> <sup>2</sup> = 8 * T(1) + 4 = 8 * 1 + 4 = 12\n",
    "\n",
    "Then asume it is true for n=2<sup>k</sup>:  \n",
    "T(2<sup>k</sup>) = (2<sup>k</sup>)<sup>2</sup> (2(2<sup>k</sup>) - 1)\n",
    "\n",
    "And want to prove that T(2<sup>k+1</sup>) = (2<sup>k+1</sup>)<sup>2</sup> * (2 * 2<sup>k+1</sup> - 1).  \n",
    "\n",
    "T(2<sup>k+1</sup>) = 8T(2<sup>k+1</sup> /2) + (2<sup>k+1</sup>)<sup>2</sup>     \n",
    "T(2<sup>k+1</sup>) = 8T(2<sup>k</sup>) + (2<sup>k+1</sup>)<sup>2</sup>     \n",
    "T(2<sup>k+1</sup>) = 8((2<sup>k</sup>)<sup>2</sup> * (2(2<sup>k</sup>) - 1)) + (2<sup>k+1</sup>)<sup>2</sup>      \n",
    "T(2<sup>k+1</sup>) = 8((2<sup>k</sup>)² * (2<sup>k+1</sup> - 1)) + (2<sup>k+1</sup>)<sup>2</sup>    \n",
    "T(2<sup>k+1</sup>) = 8(2<sup>2k</sup> * (2<sup>k+1</sup> - 1)) + (2<sup>k+1</sup>)<sup>2</sup>        \n",
    "T(2<sup>k+1</sup>) = 8(2<sup>2k</sup> * 2<sup>k+1</sup> - 2<sup>2k</sup>) + (2<sup>k+1</sup>)<sup>2</sup>  \n",
    "T(2<sup>k+1</sup>) = 2<sup>3</sup> * 2<sup>2k</sup> * 2<sup>k+1</sup> - 2<sup>3</sup> * 2<sup>2k</sup> + 2<sup>2k+2</sup>    \n",
    "T(2<sup>k+1</sup>) = 2<sup>2k+3</sup> * 2<sup>k+1</sup> - 2<sup>2k+2</sup>  \n",
    "T(2<sup>k+1</sup>) = 2<sup>3k+4</sup> - 2<sup>2k+2</sup>  \n",
    "T(2<sup>k+1</sup>) = 2<sup>2k+2</sup> * 2<sup>k+2</sup> - 2<sup>2k+2</sup>  \n",
    "T(2<sup>k+1</sup>) = 2<sup>2k+2</sup> * (2<sup>k+2</sup> - 1)   \n",
    "<u>T(2<sup>k+1</sup>) = (2<sup>k+1</sup>)<sup>2</sup> (2 * 2<sup>k+1</sup> - 1)</u>\n",
    "\n",
    "Q.E.D\n",
    "\n"
   ]
  },
  {
   "cell_type": "markdown",
   "metadata": {},
   "source": [
    "## Exercise 3\n",
    "\n",
    "\n",
    "Master theorem states that given a recurrence relation of the form:\n",
    "\n",
    "T(n) = aT(n / b) + $\\Theta$ (n<sup>d</sup>)\n",
    "\n",
    "where:  \n",
    "\"a\" is the number of subproblems in the recursion,  \n",
    "\"b\" is the factor by which the input size is reduced in each recursive call,  \n",
    "\"$\\Theta$ (n<sup>d</sup>)\" is the cost of the work done outside the recursive calls.  \n",
    "\n",
    "The Master Theorem provides asymptotic bounds for the solution \"T(n)\" based on the properties of \"$\\Theta$(n)\":\n",
    "\n",
    "If d > log_b(a):    \n",
    "Then T(n) = $\\Theta$ (n<sup>d</sup>).    \n",
    "\n",
    "If d = log_b(a):    \n",
    "Then T(n) = $\\Theta$ (n<sup>d</sup> * log(n)).  \n",
    "\n",
    "If d < log_b(a):    \n",
    "Then T(n) = $\\Theta$ (n<sup>log_b(a)</sup>).  \n",
    "\n",
    "#### a) \n",
    "T(n) = 2T(n/4) + 1\n",
    "\n",
    "Her a=2, b=4 and d=0  \n",
    "d = 0  \n",
    "log_b(a) = log_4(2) = 0.5  \n",
    "d < log_b(a)    \n",
    "T(n) = $\\Theta$ (n<sup>log_b(a)</sup>)  \n",
    "T(n) = $\\Theta$ (n<sup>log_4(2)</sup>)  \n",
    "T(n) = $\\Theta$ ($\\sqrt{n}$)\n",
    "\n",
    "#### b) \n",
    "T(n) = 2T(n/4) + sqrt(n)\n",
    "\n",
    "Her a=2, b=4 and d=0.5  \n",
    "d = log_b(a)  \n",
    "T(n) = $\\Theta$ ($\\sqrt{n}$ * log(n))\n",
    "\n",
    "#### c) \n",
    "T(n) = 2T(n/4) + n\n",
    "\n",
    "Her a=2, b=4 and d=1  \n",
    "d > log_b(a)  \n",
    "T(n) = $\\Theta$(n<sup>1</sup>)   \n",
    "T(n) = $\\Theta$(n)\n",
    "\n",
    "#### d) \n",
    "T(n) = 2T(n/4) + n<sup>2</sup>\n",
    "\n",
    "Her a=2, b=4 and d=2  \n",
    "d > log_b(a)   \n",
    "T(n) = $\\Theta$(n<sup>2</sup>)\n",
    "\n",
    "\n"
   ]
  }
 ],
 "metadata": {
  "language_info": {
   "name": "python"
  }
 },
 "nbformat": 4,
 "nbformat_minor": 2
}
