{
 "cells": [
  {
   "cell_type": "markdown",
   "metadata": {},
   "source": [
    "# Assignment 2\n",
    "\n",
    "Peder Ørmen Bukaasen, Bård Tollef Pedersen and Eivind Lid Trøen"
   ]
  },
  {
   "cell_type": "markdown",
   "metadata": {},
   "source": [
    "## Exercise 1\n"
   ]
  },
  {
   "cell_type": "markdown",
   "metadata": {},
   "source": [
    "### A\n",
    "For all positive integers n, The sum of the first n square numbers is eaual to n(n+1)(2n+1) / 6  \n",
    "\n",
    "We assume that the formula holds for some arbitrary positive integer\n",
    "1<sup>2</sup> + 2<sup>2</sup> + 3<sup>2</sup> + ... + k<sup>2</sup> = k(k+1)(2k+1) / 6 \n",
    "\n",
    "We need to show that the formula holds for n = k + 1, \n",
    "\n",
    "1<sup>2</sup> + 2<sup>2</sup> + ... + (k+1)<sup>2</sup> = (k+1)((k+1)+1)(2(k+1)+1) / 6   \n",
    "LHS = RHS\n",
    "\n",
    "Starting with the left-hand side (LHS), which is the sum of the first k+1 square numbers:\n",
    "\n",
    "LHS => 1<sup>2</sup> + 2<sup>2</sup> + ... + k<sup>2</sup> + (k+1)<sup>2</sup>\n",
    "\n",
    "We know that  1<sup>2</sup> + 2<sup>2</sup> + ... + k<sup>2</sup>  can be expressed as k(k+1)(2k+1) / 6  (our inductive hypothesis).\n",
    "So, the LHS becomes:  \n",
    "LHS = k(k+1)(2k+1) / 6  +  k<sup>2</sup>  \n",
    "LHS = (k(k+1)(2k+1) + 6(k+1)<sup>2</sup>) / 6   \n",
    "LHS = ((k+1)(k(2k+1) + 6(k+1))) / 6  \n",
    "LHS = ((k+1)(2k^2 + k + 6k + 6)) / 6   \n",
    "LHS = ((k+1)(2k^2 + 7k + 6)) / 6  \n",
    "LHS = ((k+1)(k+2)(2k+3)) / 6  \n",
    "\n",
    "RHS = (k+1)((k+1)+1)(2(k+1)+1) / 6   \n",
    "RHS = ((k+1)(k+2)(2k+3)) / 6  \n",
    "​\t\n",
    "\n",
    "The LHS is the same as the right-hand side (RHS). Thus, we've shown that if the formula holds for k, it also holds for k + 1.\n",
    "\n",
    "By the principle of mathematical induction, the formula holds for all positive integers n. Therefore, we've proven that the sum of the first n square numbers is indeed (n(n+1)(2n+1)) / 6.\n",
    "\n",
    "\n",
    "### B\n",
    "For all integers n, if n<sup>3</sup> + 5 is odd then n is even.\n",
    "\n",
    "lets say that n is even, and that measn n+1 is odd.  \n",
    "n<sup>3</sup> + 5 = n * n * n + 5 => n + 5 => n + n + 1 => n + 1 => odd\n",
    "\n",
    "No test if n is odd as n+1  \n",
    "(n+1)*(n+1)*(n+1) + 5 => n<sup>3</sup> + 3*n<sup>2</sup> + 3*n + 1  \n",
    "n<sup>3</sup> => n  \n",
    "3*n<sup>2</sup> => n   \n",
    "3*n => n + 1   \n",
    "1 => n + 1  \n",
    "n + n + n + 1 + n + 1 => 4 * n + 2 => n, wich is even.\n",
    "\n",
    "The result of n<sup>3</sup> + 5 is the oppisit of n,\n",
    "so if the result is odd then n is even, and vice versa.\n",
    "\n"
   ]
  },
  {
   "cell_type": "markdown",
   "metadata": {},
   "source": [
    "## Exercise 2"
   ]
  },
  {
   "cell_type": "code",
   "execution_count": 78,
   "metadata": {},
   "outputs": [],
   "source": [
    "def recursively_search(search_list, value, index=0, start_index=0):\n",
    "         \n",
    "    # If the current index is the value, return the index\n",
    "    if search_list[index] == value:\n",
    "        return index\n",
    "\n",
    "    # If the list is at the end, begin at the start\n",
    "    if index == len(search_list) -1:\n",
    "        index = -1 \n",
    "\n",
    "    index += 1 \n",
    "    if index == start_index:\n",
    "        return -1\n",
    "    \n",
    "    return recursively_search(search_list, value, index, start_index)"
   ]
  },
  {
   "cell_type": "code",
   "execution_count": 92,
   "metadata": {},
   "outputs": [
    {
     "ename": "IndexError",
     "evalue": "list index out of range",
     "output_type": "error",
     "traceback": [
      "\u001b[0;31m---------------------------------------------------------------------------\u001b[0m",
      "\u001b[0;31mIndexError\u001b[0m                                Traceback (most recent call last)",
      "Cell \u001b[0;32mIn[92], line 7\u001b[0m\n\u001b[1;32m      5\u001b[0m start_index \u001b[38;5;241m=\u001b[39m start\n\u001b[1;32m      6\u001b[0m value \u001b[38;5;241m=\u001b[39m \u001b[38;5;124m\"\u001b[39m\u001b[38;5;124mvalue\u001b[39m\u001b[38;5;124m\"\u001b[39m\n\u001b[0;32m----> 7\u001b[0m \u001b[43mrecursively_search\u001b[49m\u001b[43m(\u001b[49m\u001b[43mlist_number\u001b[49m\u001b[43m,\u001b[49m\u001b[43m \u001b[49m\u001b[43mvalue\u001b[49m\u001b[43m,\u001b[49m\u001b[43m \u001b[49m\u001b[43mstart\u001b[49m\u001b[43m,\u001b[49m\u001b[43m \u001b[49m\u001b[43mstart_index\u001b[49m\u001b[43m)\u001b[49m\n",
      "Cell \u001b[0;32mIn[78], line 5\u001b[0m, in \u001b[0;36mrecursively_search\u001b[0;34m(search_list, value, index, start_index)\u001b[0m\n\u001b[1;32m      1\u001b[0m \u001b[38;5;28;01mdef\u001b[39;00m \u001b[38;5;21mrecursively_search\u001b[39m(search_list, value, index\u001b[38;5;241m=\u001b[39m\u001b[38;5;241m0\u001b[39m, start_index\u001b[38;5;241m=\u001b[39m\u001b[38;5;241m0\u001b[39m):\n\u001b[1;32m      2\u001b[0m \n\u001b[1;32m      3\u001b[0m          \n\u001b[1;32m      4\u001b[0m     \u001b[38;5;66;03m# If the current index is the value, return the index\u001b[39;00m\n\u001b[0;32m----> 5\u001b[0m     \u001b[38;5;28;01mif\u001b[39;00m \u001b[43msearch_list\u001b[49m\u001b[43m[\u001b[49m\u001b[43mindex\u001b[49m\u001b[43m]\u001b[49m \u001b[38;5;241m==\u001b[39m value:\n\u001b[1;32m      6\u001b[0m         \u001b[38;5;28;01mreturn\u001b[39;00m index\n\u001b[1;32m      8\u001b[0m     \u001b[38;5;66;03m# If the list is at the end, begin at the start\u001b[39;00m\n",
      "\u001b[0;31mIndexError\u001b[0m: list index out of range"
     ]
    }
   ],
   "source": [
    "# Test in python to see that it works:\n",
    "\n",
    "list_number = [1, 2, 3, 4, \"value\", \"test\", 2.5]\n",
    "start = 7\n",
    "start_index = start\n",
    "value = \"value\"\n",
    "recursively_search(list_number, value, start, start_index) # Maybe reomve the start_index from the function call"
   ]
  },
  {
   "cell_type": "markdown",
   "metadata": {},
   "source": [
    "## Exercise 3"
   ]
  },
  {
   "cell_type": "markdown",
   "metadata": {},
   "source": [
    "From the lecture,  \n",
    "\"Sn = 1/2 * n(2a + (n − 1)d), where a is the starting value, d is the constant, n is the\n",
    "number of terms\"  \n",
    "\n",
    "With the list [-4, -1, 2, 5, ... up to 20 term],  \n",
    "we then get:  \n",
    "a = -4  \n",
    "d = 3  \n",
    "n = 20  \n",
    "\n",
    "Sn = 1/2 * n * (2 * a + (n − 1) * d)   \n",
    "Sn = 1/2 * 20 * (2*-4  + (20-1)*3)  \n",
    "Sn = 1/2 * 20 * (-8 + 57)  \n",
    "Sn = 1/2 * 980  \n",
    "Sn = <u>490</u>"
   ]
  },
  {
   "cell_type": "code",
   "execution_count": 74,
   "metadata": {},
   "outputs": [
    {
     "data": {
      "text/plain": [
       "490"
      ]
     },
     "execution_count": 74,
     "metadata": {},
     "output_type": "execute_result"
    }
   ],
   "source": [
    "# Test in python to see that the answers are the same:\n",
    "\n",
    "Sn = 0\n",
    "value = -4\n",
    "for _ in range(20):\n",
    "    Sn += value\n",
    "    value += 3\n",
    "Sn"
   ]
  }
 ],
 "metadata": {
  "kernelspec": {
   "display_name": "Python 3",
   "language": "python",
   "name": "python3"
  },
  "language_info": {
   "codemirror_mode": {
    "name": "ipython",
    "version": 3
   },
   "file_extension": ".py",
   "mimetype": "text/x-python",
   "name": "python",
   "nbconvert_exporter": "python",
   "pygments_lexer": "ipython3",
   "version": "3.9.6"
  }
 },
 "nbformat": 4,
 "nbformat_minor": 2
}
